src/theories/Sum.v
@@ -1,0 +1,93 @@
+From Equations Require Import Equations.
+Require Import Coq.Program.Equality.
+Require Import Coq.Lists.List.
+
+Require Import MirrorSolve.FirstOrder.
+Require Import MirrorSolve.HLists.
+
+Import ListNotations.
+Import HListNotations.
+
+Set Universe Polymorphism.
+Section Sum.
+
+  Variable (l: signature).
+  Variable (r: signature).
+
+  Variable (ls_eq_dec : EquivDec.EqDec l.(sig_sorts) eq).
+  Variable (rs_eq_dec : EquivDec.EqDec r.(sig_sorts) eq).
+
+  Definition sorts := (l.(sig_sorts) + r.(sig_sorts))%type.
+
+  Definition sorts_eq_dec : EquivDec.EqDec sorts eq := sum_eqdec ls_eq_dec rs_eq_dec.
+
+  Set Universe Polymorphism.
+
+  Inductive funs : arity sorts -> sorts -> Type := 
+  | LFun : forall {lsa lsr}, 
+    l.(sig_funs) lsa lsr -> 
+    funs (map inl lsa) (inl lsr)
+  | RFun : forall {rsa rsr}, 
+    r.(sig_funs) rsa rsr -> 
+    funs (map inr rsa) (inr rsr).
+
+  Inductive rels: arity sorts -> Type :=
+  | LRel : forall {lsa}, 
+    l.(sig_rels) lsa -> 
+    rels (map inl lsa)
+  | RRel : forall {rsa}, 
+    r.(sig_rels) rsa -> 
+    rels (map inr rsa).
+
+  Definition sig: signature :=
+    {| sig_sorts := sorts;
+      sig_funs := funs;
+      sig_rels := rels |}.
+
+  Definition fm ctx := FirstOrder.fm sig ctx.
+  Definition tm ctx := FirstOrder.tm sig ctx.
+
+  Variable (mod_l : model l).
+  Variable (mod_r : model r).
+
+  Definition mod_sorts (s: sig_sorts sig) : Type :=
+    match s with
+    | inl sl => mod_l.(mod_sorts _) sl
+    | inr sr => mod_r.(mod_sorts _) sr
+    end.
+
+  Equations strip_hl_inl {L R} {f: (L + R)%type -> Type} (x: list L) (args: HList.t f (map inl x)) : HList.t (fun x => f (inl x)) x := 
+  { 
+    strip_hl_inl nil hnil := hnil;
+    strip_hl_inl (x :: xs) (v ::: vs) := v ::: strip_hl_inl xs vs;
+  }.
+
+  Equations strip_hl_inr {L R} {f: (L + R)%type -> Type} (x: list R) (args: HList.t f (map inr x)) : HList.t (fun x => f (inr x)) x := 
+  { 
+    strip_hl_inr nil hnil := hnil;
+    strip_hl_inr (x :: xs) (v ::: vs) := v ::: strip_hl_inr xs vs;
+  }.
+
+  Arguments strip_hl_inl {_ _ _ _} _.
+  Arguments strip_hl_inr {_ _ _ _} _.
+
+  Definition mod_fns params ret (f: sig_funs sig params ret) (args: HList.t mod_sorts params) :=
+    match f in funs a s return HList.t mod_sorts a -> mod_sorts s with 
+    | LFun f' => fun args' => mod_fns _ _ _ _ f' (strip_hl_inl args')
+    | RFun f' => fun args' => mod_fns _ _ _ _ f' (strip_hl_inr args')
+    end args.
+
+  Definition mod_rels params (f: sig_rels sig params) (args: HList.t mod_sorts params) : Prop :=
+    match f in rels a return HList.t mod_sorts a -> Prop with 
+    | LRel f' => fun args' => mod_rels _ _ _ f' (strip_hl_inl args')
+    | RRel f' => fun args' => mod_rels _ _ _ f' (strip_hl_inr args')
+    end args.
+
+  Definition fm_model : model sig := {|
+    FirstOrder.mod_sorts := mod_sorts;
+    FirstOrder.mod_fns := mod_fns;
+    FirstOrder.mod_rels := mod_rels;
+  |}.
+
+End Sum.
+
